lib.v
@@ -1,0 +1,17 @@
+(** Solve by inversion,
+    taken from SfLib.v of Software Foundation book *)
+
+Tactic Notation "solve_by_inversion_step" tactic(t) :=
+  match goal with
+  | H : _ |- _ => solve [ inversion H; subst; t ]
+  end
+  || fail "because the goal is not solvable by inversion.".
+
+Tactic Notation "solve" "by" "inversion" "1" :=
+  solve_by_inversion_step idtac.
+Tactic Notation "solve" "by" "inversion" "2" :=
+  solve_by_inversion_step (solve by inversion 1).
+Tactic Notation "solve" "by" "inversion" "3" :=
+  solve_by_inversion_step (solve by inversion 2).
+Tactic Notation "solve" "by" "inversion" :=
+  solve by inversion 1.
